<?xml version="1.0"?>
<rdf:RDF xmlns="http://www.semanticweb.org/hmoudden/ontologies/2022/10/tp01#"
     xml:base="http://www.semanticweb.org/hmoudden/ontologies/2022/10/tp01"
     xmlns:owl="http://www.w3.org/2002/07/owl#"
     xmlns:rdf="http://www.w3.org/1999/02/22-rdf-syntax-ns#"
     xmlns:xml="http://www.w3.org/XML/1998/namespace"
     xmlns:xsd="http://www.w3.org/2001/XMLSchema#"
     xmlns:rdfs="http://www.w3.org/2000/01/rdf-schema#">
    <owl:Ontology rdf:about="http://www.semanticweb.org/hmoudden/ontologies/2022/10/tp01"/>
    


    <!-- 
    ///////////////////////////////////////////////////////////////////////////////////////
    //
    // Object Properties
    //
    ///////////////////////////////////////////////////////////////////////////////////////
     -->

    


    <!-- http://www.semanticweb.org/hmoudden/ontologies/2022/10/tp01#aCapitale -->

    <owl:ObjectProperty rdf:about="http://www.semanticweb.org/hmoudden/ontologies/2022/10/tp01#aCapitale">
        <rdfs:subPropertyOf rdf:resource="http://www.semanticweb.org/hmoudden/ontologies/2022/10/tp01#contient"/>
        <rdfs:domain rdf:resource="http://www.semanticweb.org/hmoudden/ontologies/2022/10/tp01#Lieu"/>
        <rdfs:range rdf:resource="http://www.semanticweb.org/hmoudden/ontologies/2022/10/tp01#Lieu"/>
        <rdfs:comment xml:lang="en">hasCapitale is an object property which means that a country has a capital city.
If a country has a city as its capital, then this country contains this city.</rdfs:comment>
        <rdfs:label xml:lang="fr">aCapitale</rdfs:label>
        <rdfs:label xml:lang="en">hasCapitale</rdfs:label>
    </owl:ObjectProperty>
    


    <!-- http://www.semanticweb.org/hmoudden/ontologies/2022/10/tp01#aCommeActeur -->

    <owl:ObjectProperty rdf:about="http://www.semanticweb.org/hmoudden/ontologies/2022/10/tp01#aCommeActeur">
        <owl:inverseOf rdf:resource="http://www.semanticweb.org/hmoudden/ontologies/2022/10/tp01#joueDansFilm"/>
        <rdfs:domain rdf:resource="http://www.semanticweb.org/hmoudden/ontologies/2022/10/tp01#Film"/>
        <rdfs:range rdf:resource="http://www.semanticweb.org/hmoudden/ontologies/2022/10/tp01#Artiste"/>
        <rdfs:comment xml:lang="en">asActor is an object property to say that a movie given to one or more artists.
This property is the inverse of playInMovie.</rdfs:comment>
        <rdfs:label xml:lang="fr">aCommeActeur</rdfs:label>
        <rdfs:label xml:lang="en">asActor</rdfs:label>
    </owl:ObjectProperty>
    


    <!-- http://www.semanticweb.org/hmoudden/ontologies/2022/10/tp01#aGenre -->

    <owl:ObjectProperty rdf:about="http://www.semanticweb.org/hmoudden/ontologies/2022/10/tp01#aGenre">
        <rdfs:subPropertyOf rdf:resource="http://www.w3.org/2002/07/owl#topObjectProperty"/>
        <rdfs:domain rdf:resource="http://www.semanticweb.org/hmoudden/ontologies/2022/10/tp01#Personne"/>
        <rdfs:range rdf:resource="http://www.semanticweb.org/hmoudden/ontologies/2022/10/tp01#Genre"/>
        <rdfs:comment xml:lang="en">hasGender is an object property to say that a person must have only one gender.</rdfs:comment>
        <rdfs:label xml:lang="fr">aGenre</rdfs:label>
        <rdfs:label xml:lang="en">hasGender</rdfs:label>
    </owl:ObjectProperty>
    


    <!-- http://www.semanticweb.org/hmoudden/ontologies/2022/10/tp01#aNationalité -->

    <owl:ObjectProperty rdf:about="http://www.semanticweb.org/hmoudden/ontologies/2022/10/tp01#aNationalité">
        <rdfs:subPropertyOf rdf:resource="http://www.w3.org/2002/07/owl#topObjectProperty"/>
        <rdfs:domain rdf:resource="http://www.semanticweb.org/hmoudden/ontologies/2022/10/tp01#Film"/>
        <rdfs:range rdf:resource="http://www.semanticweb.org/hmoudden/ontologies/2022/10/tp01#Nationalité"/>
        <rdfs:comment xml:lang="en">hasNationality is an object property to say that a movie has a nationality.</rdfs:comment>
        <rdfs:label xml:lang="fr">aNationalité</rdfs:label>
        <rdfs:label xml:lang="en">hasNationality</rdfs:label>
    </owl:ObjectProperty>
    


    <!-- http://www.semanticweb.org/hmoudden/ontologies/2022/10/tp01#aRéalisé -->

    <owl:ObjectProperty rdf:about="http://www.semanticweb.org/hmoudden/ontologies/2022/10/tp01#aRéalisé">
        <rdfs:subPropertyOf rdf:resource="http://www.w3.org/2002/07/owl#topObjectProperty"/>
        <owl:inverseOf rdf:resource="http://www.semanticweb.org/hmoudden/ontologies/2022/10/tp01#réaliséPar"/>
        <rdfs:domain rdf:resource="http://www.semanticweb.org/hmoudden/ontologies/2022/10/tp01#Réalisateur"/>
        <rdfs:range rdf:resource="http://www.semanticweb.org/hmoudden/ontologies/2022/10/tp01#Film"/>
        <rdfs:comment xml:lang="en">hasDirected is an object property to designate that a director has directed a film.</rdfs:comment>
        <rdfs:label xml:lang="fr">aRéalisé</rdfs:label>
        <rdfs:label xml:lang="en">hasDirected</rdfs:label>
    </owl:ObjectProperty>
    


    <!-- http://www.semanticweb.org/hmoudden/ontologies/2022/10/tp01#contient -->

    <owl:ObjectProperty rdf:about="http://www.semanticweb.org/hmoudden/ontologies/2022/10/tp01#contient">
        <owl:inverseOf rdf:resource="http://www.semanticweb.org/hmoudden/ontologies/2022/10/tp01#situéDans"/>
        <rdf:type rdf:resource="http://www.w3.org/2002/07/owl#TransitiveProperty"/>
        <rdfs:domain rdf:resource="http://www.semanticweb.org/hmoudden/ontologies/2022/10/tp01#Lieu"/>
        <rdfs:range rdf:resource="http://www.semanticweb.org/hmoudden/ontologies/2022/10/tp01#Lieu"/>
        <rdfs:comment xml:lang="en">contains is an object property that means that a place contains another place.
Thanks to the transitivity of the relation Contains, the reasoner knows that if a place A is located in a place B and this place B is located in a place C, then the place A is located in the place C
This property is the inverse of locatedIn.</rdfs:comment>
        <rdfs:label xml:lang="en">contains</rdfs:label>
        <rdfs:label xml:lang="fr">contient</rdfs:label>
    </owl:ObjectProperty>
    


    <!-- http://www.semanticweb.org/hmoudden/ontologies/2022/10/tp01#joueDansFilm -->

    <owl:ObjectProperty rdf:about="http://www.semanticweb.org/hmoudden/ontologies/2022/10/tp01#joueDansFilm">
        <rdfs:subPropertyOf rdf:resource="http://www.w3.org/2002/07/owl#topObjectProperty"/>
        <rdfs:domain rdf:resource="http://www.semanticweb.org/hmoudden/ontologies/2022/10/tp01#Artiste"/>
        <rdfs:range rdf:resource="http://www.semanticweb.org/hmoudden/ontologies/2022/10/tp01#Film"/>
        <rdfs:comment xml:lang="en">playInMovie is an object property to say that a given artist has acted in a movie.
This property is the inverse of asActor.</rdfs:comment>
        <rdfs:label xml:lang="fr">joueDansFilm</rdfs:label>
        <rdfs:label xml:lang="en">playsInMovie</rdfs:label>
    </owl:ObjectProperty>
    


    <!-- http://www.semanticweb.org/hmoudden/ontologies/2022/10/tp01#réaliséPar -->

    <owl:ObjectProperty rdf:about="http://www.semanticweb.org/hmoudden/ontologies/2022/10/tp01#réaliséPar">
        <rdfs:subPropertyOf rdf:resource="http://www.w3.org/2002/07/owl#topObjectProperty"/>
        <rdfs:domain rdf:resource="http://www.semanticweb.org/hmoudden/ontologies/2022/10/tp01#Film"/>
        <rdfs:range rdf:resource="http://www.semanticweb.org/hmoudden/ontologies/2022/10/tp01#Réalisateur"/>
        <rdfs:comment xml:lang="en">isDirectedBy is an object property to designate that a film is directed by a director.
This property is the inverse of hasDirected.</rdfs:comment>
        <rdfs:label xml:lang="en">isDirectedBy</rdfs:label>
        <rdfs:label xml:lang="fr">réaliséPar</rdfs:label>
    </owl:ObjectProperty>
    


    <!-- http://www.semanticweb.org/hmoudden/ontologies/2022/10/tp01#seDérouleDans -->

    <owl:ObjectProperty rdf:about="http://www.semanticweb.org/hmoudden/ontologies/2022/10/tp01#seDérouleDans">
        <rdfs:subPropertyOf rdf:resource="http://www.w3.org/2002/07/owl#topObjectProperty"/>
        <rdfs:domain rdf:resource="http://www.semanticweb.org/hmoudden/ontologies/2022/10/tp01#Film"/>
        <rdfs:range rdf:resource="http://www.semanticweb.org/hmoudden/ontologies/2022/10/tp01#Lieu"/>
        <owl:propertyChainAxiom rdf:parseType="Collection">
            <rdf:Description rdf:about="http://www.semanticweb.org/hmoudden/ontologies/2022/10/tp01#seDérouleDans"/>
            <rdf:Description rdf:about="http://www.semanticweb.org/hmoudden/ontologies/2022/10/tp01#situéDans"/>
        </owl:propertyChainAxiom>
        <rdfs:comment xml:lang="en">takesPlaceIn is an object property that means a movie takes place in a given location.
The reasoner also deduces that the film Midnight in Paris took place in France and in Europe since we informed that the film took place in Paris.</rdfs:comment>
        <rdfs:label xml:lang="fr">seDérouleDans</rdfs:label>
        <rdfs:label xml:lang="en">takePlaceIn</rdfs:label>
    </owl:ObjectProperty>
    


    <!-- http://www.semanticweb.org/hmoudden/ontologies/2022/10/tp01#situéDans -->

    <owl:ObjectProperty rdf:about="http://www.semanticweb.org/hmoudden/ontologies/2022/10/tp01#situéDans">
        <rdfs:subPropertyOf rdf:resource="http://www.w3.org/2002/07/owl#topObjectProperty"/>
        <rdfs:domain rdf:resource="http://www.semanticweb.org/hmoudden/ontologies/2022/10/tp01#Lieu"/>
        <rdfs:range rdf:resource="http://www.semanticweb.org/hmoudden/ontologies/2022/10/tp01#Lieu"/>
        <rdfs:comment xml:lang="en">locatedIn is an object property which means that a place is located in another place.
This property is the inverse of contains.</rdfs:comment>
        <rdfs:label xml:lang="en">locatedIn</rdfs:label>
        <rdfs:label xml:lang="fr">situéDans</rdfs:label>
    </owl:ObjectProperty>
    


    <!-- 
    ///////////////////////////////////////////////////////////////////////////////////////
    //
    // Data properties
    //
    ///////////////////////////////////////////////////////////////////////////////////////
     -->

    


    <!-- http://www.semanticweb.org/hmoudden/ontologies/2022/10/tp01#Durée -->

    <owl:DatatypeProperty rdf:about="http://www.semanticweb.org/hmoudden/ontologies/2022/10/tp01#Durée">
        <rdfs:domain rdf:resource="http://www.semanticweb.org/hmoudden/ontologies/2022/10/tp01#Film"/>
        <rdfs:range rdf:resource="http://www.w3.org/2001/XMLSchema#int"/>
        <rdfs:comment xml:lang="en">Duration is a data object of type xsd:integer associated with a movie which designates the number of minutes of a movie</rdfs:comment>
        <rdfs:label xml:lang="en">Duration</rdfs:label>
        <rdfs:label xml:lang="fr">Durée</rdfs:label>
    </owl:DatatypeProperty>
    


    <!-- http://www.semanticweb.org/hmoudden/ontologies/2022/10/tp01#Note -->

    <owl:DatatypeProperty rdf:about="http://www.semanticweb.org/hmoudden/ontologies/2022/10/tp01#Note">
        <rdfs:domain rdf:resource="http://www.semanticweb.org/hmoudden/ontologies/2022/10/tp01#Film"/>
        <rdfs:range rdf:resource="http://www.w3.org/1999/02/22-rdf-syntax-ns#PlainLiteral"/>
        <rdfs:comment xml:lang="en">Note is a data object of type ref:PlainLiteral associated with a given movie which designates a summary description of the movie.</rdfs:comment>
        <rdfs:label xml:lang="fr">Note</rdfs:label>
        <rdfs:label xml:lang="en">Summary</rdfs:label>
    </owl:DatatypeProperty>
    


    <!-- 
    ///////////////////////////////////////////////////////////////////////////////////////
    //
    // Classes
    //
    ///////////////////////////////////////////////////////////////////////////////////////
     -->

    


    <!-- http://www.semanticweb.org/hmoudden/ontologies/2022/10/tp01#Acteur -->

    <owl:Class rdf:about="http://www.semanticweb.org/hmoudden/ontologies/2022/10/tp01#Acteur">
        <owl:equivalentClass>
            <owl:Class>
                <owl:intersectionOf rdf:parseType="Collection">
                    <rdf:Description rdf:about="http://www.semanticweb.org/hmoudden/ontologies/2022/10/tp01#Artiste"/>
                    <owl:Restriction>
                        <owl:onProperty rdf:resource="http://www.semanticweb.org/hmoudden/ontologies/2022/10/tp01#aGenre"/>
                        <owl:hasValue rdf:resource="http://www.semanticweb.org/hmoudden/ontologies/2022/10/tp01#Masculin"/>
                    </owl:Restriction>
                </owl:intersectionOf>
            </owl:Class>
        </owl:equivalentClass>
        <rdfs:subClassOf rdf:resource="http://www.semanticweb.org/hmoudden/ontologies/2022/10/tp01#Artiste"/>
        <rdfs:comment xml:lang="fr">This is a person of male gender who has played in one or more films.
This makes it possible to have the property of playsInMovie.
As Actress is a subclass of Person, it inherited the object property hasGender which is set to Man for this class.
As well as this class allows to have labels by languages and comments for each subclass.</rdfs:comment>
        <rdfs:label xml:lang="en">Actor</rdfs:label>
        <rdfs:label xml:lang="fr">Comédien</rdfs:label>
    </owl:Class>
    


    <!-- http://www.semanticweb.org/hmoudden/ontologies/2022/10/tp01#Actrice -->

    <owl:Class rdf:about="http://www.semanticweb.org/hmoudden/ontologies/2022/10/tp01#Actrice">
        <owl:equivalentClass>
            <owl:Class>
                <owl:intersectionOf rdf:parseType="Collection">
                    <rdf:Description rdf:about="http://www.semanticweb.org/hmoudden/ontologies/2022/10/tp01#Artiste"/>
                    <owl:Restriction>
                        <owl:onProperty rdf:resource="http://www.semanticweb.org/hmoudden/ontologies/2022/10/tp01#aGenre"/>
                        <owl:hasValue rdf:resource="http://www.semanticweb.org/hmoudden/ontologies/2022/10/tp01#Féminin"/>
                    </owl:Restriction>
                </owl:intersectionOf>
            </owl:Class>
        </owl:equivalentClass>
        <rdfs:subClassOf rdf:resource="http://www.semanticweb.org/hmoudden/ontologies/2022/10/tp01#Artiste"/>
        <rdfs:comment xml:lang="en">This is a person of female gender who has played in one or more films.
This makes it possible to have the property of playsInMovie.
As Actress is a subclass of Person, it inherited the object property hasGender which is set to Woman for this class.
As well as this class allows to have labels by languages and comments for each subclass.</rdfs:comment>
        <rdfs:label xml:lang="en">Actress</rdfs:label>
        <rdfs:label xml:lang="fr">Comédienne</rdfs:label>
    </owl:Class>
    


    <!-- http://www.semanticweb.org/hmoudden/ontologies/2022/10/tp01#Artiste -->

    <owl:Class rdf:about="http://www.semanticweb.org/hmoudden/ontologies/2022/10/tp01#Artiste">
        <rdfs:subClassOf rdf:resource="http://www.semanticweb.org/hmoudden/ontologies/2022/10/tp01#Personne"/>
        <rdfs:subClassOf>
            <owl:Restriction>
                <owl:onProperty rdf:resource="http://www.semanticweb.org/hmoudden/ontologies/2022/10/tp01#joueDansFilm"/>
                <owl:someValuesFrom rdf:resource="http://www.semanticweb.org/hmoudden/ontologies/2022/10/tp01#Film"/>
            </owl:Restriction>
        </rdfs:subClassOf>
        <rdfs:comment xml:lang="en">This is a person who has acted in one or more films.
An artist has necessarily played in one or more films.
As Artist is a subclass of Person, it inherited the hasGender property.
As well as this class allows to have labels by languages and comments for each subclass.</rdfs:comment>
        <rdfs:label xml:lang="en">Artist</rdfs:label>
        <rdfs:label xml:lang="fr">Artiste</rdfs:label>
    </owl:Class>
    


    <!-- http://www.semanticweb.org/hmoudden/ontologies/2022/10/tp01#Continent -->

    <owl:Class rdf:about="http://www.semanticweb.org/hmoudden/ontologies/2022/10/tp01#Continent">
        <rdfs:subClassOf rdf:resource="http://www.semanticweb.org/hmoudden/ontologies/2022/10/tp01#Lieu"/>
        <owl:disjointWith rdf:resource="http://www.semanticweb.org/hmoudden/ontologies/2022/10/tp01#Pays"/>
        <owl:disjointWith rdf:resource="http://www.semanticweb.org/hmoudden/ontologies/2022/10/tp01#Ville"/>
        <rdfs:comment xml:lang="en">The Continent is declared as an equivalence class to avoid that a place equivalent to a contains is not.
As well as this class allows to have labels by languages.
This class is disjoint with the Country and City class, which means that a Continent cannot be a Country or a City.</rdfs:comment>
        <rdfs:label xml:lang="en">Continent</rdfs:label>
        <rdfs:label xml:lang="fr">Continent</rdfs:label>
    </owl:Class>
    


    <!-- http://www.semanticweb.org/hmoudden/ontologies/2022/10/tp01#Court-Métrage -->

    <owl:Class rdf:about="http://www.semanticweb.org/hmoudden/ontologies/2022/10/tp01#Court-Métrage">
        <owl:equivalentClass>
            <owl:Class>
                <owl:intersectionOf rdf:parseType="Collection">
                    <rdf:Description rdf:about="http://www.semanticweb.org/hmoudden/ontologies/2022/10/tp01#Film"/>
                    <owl:Restriction>
                        <owl:onProperty rdf:resource="http://www.semanticweb.org/hmoudden/ontologies/2022/10/tp01#Durée"/>
                        <owl:someValuesFrom>
                            <rdfs:Datatype>
                                <owl:onDatatype rdf:resource="http://www.w3.org/2001/XMLSchema#int"/>
                                <owl:withRestrictions rdf:parseType="Collection">
                                    <rdf:Description>
                                        <xsd:maxExclusive rdf:datatype="http://www.w3.org/2001/XMLSchema#int">59</xsd:maxExclusive>
                                    </rdf:Description>
                                </owl:withRestrictions>
                            </rdfs:Datatype>
                        </owl:someValuesFrom>
                    </owl:Restriction>
                </owl:intersectionOf>
            </owl:Class>
        </owl:equivalentClass>
        <rdfs:subClassOf rdf:resource="http://www.semanticweb.org/hmoudden/ontologies/2022/10/tp01#Film"/>
        <owl:disjointWith rdf:resource="http://www.semanticweb.org/hmoudden/ontologies/2022/10/tp01#Long-Métrage"/>
        <rdfs:comment xml:lang="en">It is a film whose duration is less than 60 minutes.
It inherits all the properties of the Movie class.
As well as this class allows to have labels by languages.
This class is separate from the Feature-Film class, which means that a Short-Film cannot be a Feature-Film.</rdfs:comment>
        <rdfs:label xml:lang="fr">Court métrage</rdfs:label>
        <rdfs:label xml:lang="en">Short film</rdfs:label>
    </owl:Class>
    


    <!-- http://www.semanticweb.org/hmoudden/ontologies/2022/10/tp01#Femme -->

    <owl:Class rdf:about="http://www.semanticweb.org/hmoudden/ontologies/2022/10/tp01#Femme">
        <owl:equivalentClass>
            <owl:Class>
                <owl:intersectionOf rdf:parseType="Collection">
                    <rdf:Description rdf:about="http://www.semanticweb.org/hmoudden/ontologies/2022/10/tp01#Personne"/>
                    <owl:Restriction>
                        <owl:onProperty rdf:resource="http://www.semanticweb.org/hmoudden/ontologies/2022/10/tp01#aGenre"/>
                        <owl:hasValue rdf:resource="http://www.semanticweb.org/hmoudden/ontologies/2022/10/tp01#Féminin"/>
                    </owl:Restriction>
                </owl:intersectionOf>
            </owl:Class>
        </owl:equivalentClass>
        <rdfs:subClassOf rdf:resource="http://www.semanticweb.org/hmoudden/ontologies/2022/10/tp01#Personne"/>
        <rdfs:comment xml:lang="en">Woman is a person with a Female gender.
Since Woman is a subclass of Person, it inherits the hasGender object property.
As well as this class allows to have labels by languages and comments for each subclass.</rdfs:comment>
        <rdfs:label xml:lang="fr">Femme</rdfs:label>
        <rdfs:label xml:lang="en">Women</rdfs:label>
    </owl:Class>
    


    <!-- http://www.semanticweb.org/hmoudden/ontologies/2022/10/tp01#Film -->

    <owl:Class rdf:about="http://www.semanticweb.org/hmoudden/ontologies/2022/10/tp01#Film">
        <rdfs:subClassOf>
            <owl:Restriction>
                <owl:onProperty rdf:resource="http://www.semanticweb.org/hmoudden/ontologies/2022/10/tp01#aNationalité"/>
                <owl:someValuesFrom rdf:resource="http://www.semanticweb.org/hmoudden/ontologies/2022/10/tp01#Nationalité"/>
            </owl:Restriction>
        </rdfs:subClassOf>
        <rdfs:subClassOf>
            <owl:Restriction>
                <owl:onProperty rdf:resource="http://www.semanticweb.org/hmoudden/ontologies/2022/10/tp01#réaliséPar"/>
                <owl:someValuesFrom rdf:resource="http://www.semanticweb.org/hmoudden/ontologies/2022/10/tp01#Réalisateur"/>
            </owl:Restriction>
        </rdfs:subClassOf>
        <rdfs:subClassOf>
            <owl:Restriction>
                <owl:onProperty rdf:resource="http://www.semanticweb.org/hmoudden/ontologies/2022/10/tp01#seDérouleDans"/>
                <owl:someValuesFrom rdf:resource="http://www.semanticweb.org/hmoudden/ontologies/2022/10/tp01#Lieu"/>
            </owl:Restriction>
        </rdfs:subClassOf>
        <rdfs:subClassOf>
            <owl:Restriction>
                <owl:onProperty rdf:resource="http://www.semanticweb.org/hmoudden/ontologies/2022/10/tp01#Durée"/>
                <owl:qualifiedCardinality rdf:datatype="http://www.w3.org/2001/XMLSchema#nonNegativeInteger">1</owl:qualifiedCardinality>
                <owl:onDataRange rdf:resource="http://www.w3.org/2001/XMLSchema#integer"/>
            </owl:Restriction>
        </rdfs:subClassOf>
        <rdfs:subClassOf>
            <owl:Restriction>
                <owl:onProperty rdf:resource="http://www.semanticweb.org/hmoudden/ontologies/2022/10/tp01#Note"/>
                <owl:qualifiedCardinality rdf:datatype="http://www.w3.org/2001/XMLSchema#nonNegativeInteger">1</owl:qualifiedCardinality>
                <owl:onDataRange rdf:resource="http://www.w3.org/1999/02/22-rdf-syntax-ns#PlainLiteral"/>
            </owl:Restriction>
        </rdfs:subClassOf>
        <rdfs:comment xml:lang="en">Film is declared as a class such that a film contains different types of films.
This allows having multiple object properties like aNationality, DoneBy, and OccursIn, as well as having given properties like duration and rating.
As well as this class allows to have labels by languages and comments for each subclass.</rdfs:comment>
        <rdfs:label xml:lang="fr">Film</rdfs:label>
        <rdfs:label xml:lang="en">Movie</rdfs:label>
    </owl:Class>
    


    <!-- http://www.semanticweb.org/hmoudden/ontologies/2022/10/tp01#Film-Européen -->

    <owl:Class rdf:about="http://www.semanticweb.org/hmoudden/ontologies/2022/10/tp01#Film-Européen">
        <owl:equivalentClass>
            <owl:Restriction>
                <owl:onProperty rdf:resource="http://www.semanticweb.org/hmoudden/ontologies/2022/10/tp01#aNationalité"/>
                <owl:hasValue rdf:resource="http://www.semanticweb.org/hmoudden/ontologies/2022/10/tp01#Français"/>
            </owl:Restriction>
        </owl:equivalentClass>
        <rdfs:subClassOf rdf:resource="http://www.semanticweb.org/hmoudden/ontologies/2022/10/tp01#Film"/>
        <rdfs:comment xml:lang="en">It is a class of film whose nationality is associated with a European country.
It inherits all the properties of the Movie class.
As well as this class allows to have labels by languages.</rdfs:comment>
        <rdfs:label xml:lang="en">European movie</rdfs:label>
        <rdfs:label xml:lang="fr">Film Européen</rdfs:label>
    </owl:Class>
    


    <!-- http://www.semanticweb.org/hmoudden/ontologies/2022/10/tp01#Genre -->

    <owl:Class rdf:about="http://www.semanticweb.org/hmoudden/ontologies/2022/10/tp01#Genre">
        <rdfs:comment xml:lang="en">The gender is declared as a class with instances to be able to modify the list of possible instances as needed (Male, Female).
This allows to have an aGenre property and perform tests on its value.
It also allows to have the labels by languages and comments for each gender instance.</rdfs:comment>
        <rdfs:label xml:lang="en">Gender</rdfs:label>
        <rdfs:label xml:lang="fr">Genre</rdfs:label>
    </owl:Class>
    


    <!-- http://www.semanticweb.org/hmoudden/ontologies/2022/10/tp01#Homme -->

    <owl:Class rdf:about="http://www.semanticweb.org/hmoudden/ontologies/2022/10/tp01#Homme">
        <owl:equivalentClass>
            <owl:Class>
                <owl:intersectionOf rdf:parseType="Collection">
                    <rdf:Description rdf:about="http://www.semanticweb.org/hmoudden/ontologies/2022/10/tp01#Personne"/>
                    <owl:Restriction>
                        <owl:onProperty rdf:resource="http://www.semanticweb.org/hmoudden/ontologies/2022/10/tp01#aGenre"/>
                        <owl:hasValue rdf:resource="http://www.semanticweb.org/hmoudden/ontologies/2022/10/tp01#Masculin"/>
                    </owl:Restriction>
                </owl:intersectionOf>
            </owl:Class>
        </owl:equivalentClass>
        <rdfs:subClassOf rdf:resource="http://www.semanticweb.org/hmoudden/ontologies/2022/10/tp01#Personne"/>
        <rdfs:comment xml:lang="en">Man is a person with a Male gender.
Since Man is a subclass of Person, it inherits the hasGender object property.
As well as this class allows to have labels by languages and comments for each subclass.</rdfs:comment>
        <rdfs:label xml:lang="fr">Homme</rdfs:label>
        <rdfs:label xml:lang="en">Man</rdfs:label>
    </owl:Class>
    


    <!-- http://www.semanticweb.org/hmoudden/ontologies/2022/10/tp01#Lieu -->

    <owl:Class rdf:about="http://www.semanticweb.org/hmoudden/ontologies/2022/10/tp01#Lieu">
        <rdfs:subClassOf>
            <owl:Restriction>
                <owl:onProperty rdf:resource="http://www.semanticweb.org/hmoudden/ontologies/2022/10/tp01#situéDans"/>
                <owl:someValuesFrom rdf:resource="http://www.semanticweb.org/hmoudden/ontologies/2022/10/tp01#Lieu"/>
            </owl:Restriction>
        </rdfs:subClassOf>
        <rdfs:comment xml:lang="en">The Location is a class that a Location is a city, a country or a continent.
This makes it possible to have an object property locatedIn.
As well as this class allows to have labels by languages and comments for each subclass.</rdfs:comment>
        <rdfs:label xml:lang="fr">Lieu</rdfs:label>
        <rdfs:label xml:lang="en">Place</rdfs:label>
    </owl:Class>
    


    <!-- http://www.semanticweb.org/hmoudden/ontologies/2022/10/tp01#Long-Métrage -->

    <owl:Class rdf:about="http://www.semanticweb.org/hmoudden/ontologies/2022/10/tp01#Long-Métrage">
        <owl:equivalentClass>
            <owl:Class>
                <owl:intersectionOf rdf:parseType="Collection">
                    <rdf:Description rdf:about="http://www.semanticweb.org/hmoudden/ontologies/2022/10/tp01#Film"/>
                    <owl:Restriction>
                        <owl:onProperty rdf:resource="http://www.semanticweb.org/hmoudden/ontologies/2022/10/tp01#Durée"/>
                        <owl:someValuesFrom>
                            <rdfs:Datatype>
                                <owl:onDatatype rdf:resource="http://www.w3.org/2001/XMLSchema#int"/>
                                <owl:withRestrictions rdf:parseType="Collection">
                                    <rdf:Description>
                                        <xsd:minExclusive rdf:datatype="http://www.w3.org/2001/XMLSchema#int">59</xsd:minExclusive>
                                    </rdf:Description>
                                </owl:withRestrictions>
                            </rdfs:Datatype>
                        </owl:someValuesFrom>
                    </owl:Restriction>
                </owl:intersectionOf>
            </owl:Class>
        </owl:equivalentClass>
        <rdfs:subClassOf rdf:resource="http://www.semanticweb.org/hmoudden/ontologies/2022/10/tp01#Film"/>
        <rdfs:comment xml:lang="en">It is a film whose duration is greater than or equal to 60 minutes.
It inherits all the properties of the Movie class.
As well as this class allows to have labels by languages.
This class is separate from the Short-Film class, which means that a Feature-Film cannot be a Short-Film</rdfs:comment>
        <rdfs:label xml:lang="en">Feature film</rdfs:label>
        <rdfs:label xml:lang="fr">Long métrage</rdfs:label>
    </owl:Class>
    


    <!-- http://www.semanticweb.org/hmoudden/ontologies/2022/10/tp01#Nationalité -->

    <owl:Class rdf:about="http://www.semanticweb.org/hmoudden/ontologies/2022/10/tp01#Nationalité">
        <rdfs:comment xml:lang="en">Nationality is a class with instances to be able to modify the list of possible instances (French) as needed.
It also allows to have the labels by languages and comments for each gender instance.</rdfs:comment>
        <rdfs:label xml:lang="en">Nationality</rdfs:label>
        <rdfs:label xml:lang="fr">Nationalité</rdfs:label>
    </owl:Class>
    


    <!-- http://www.semanticweb.org/hmoudden/ontologies/2022/10/tp01#Pays -->

    <owl:Class rdf:about="http://www.semanticweb.org/hmoudden/ontologies/2022/10/tp01#Pays">
        <rdfs:subClassOf rdf:resource="http://www.semanticweb.org/hmoudden/ontologies/2022/10/tp01#Lieu"/>
        <rdfs:subClassOf>
            <owl:Restriction>
                <owl:onProperty rdf:resource="http://www.semanticweb.org/hmoudden/ontologies/2022/10/tp01#aCapitale"/>
                <owl:qualifiedCardinality rdf:datatype="http://www.w3.org/2001/XMLSchema#nonNegativeInteger">1</owl:qualifiedCardinality>
                <owl:onClass rdf:resource="http://www.semanticweb.org/hmoudden/ontologies/2022/10/tp01#Ville"/>
            </owl:Restriction>
        </rdfs:subClassOf>
        <owl:disjointWith rdf:resource="http://www.semanticweb.org/hmoudden/ontologies/2022/10/tp01#Ville"/>
        <rdfs:comment xml:lang="en">The Country is declared as an equivalence class to avoid that a place equivalent to a country is not.
As well as this class allows to have labels by languages.
This class is disjoint with the Continent and City class, which means that a Country cannot be a Continent or a City.</rdfs:comment>
        <rdfs:label xml:lang="en">Country</rdfs:label>
        <rdfs:label xml:lang="fr">Pays</rdfs:label>
    </owl:Class>
    


    <!-- http://www.semanticweb.org/hmoudden/ontologies/2022/10/tp01#Personne -->

    <owl:Class rdf:about="http://www.semanticweb.org/hmoudden/ontologies/2022/10/tp01#Personne">
        <rdfs:subClassOf>
            <owl:Restriction>
                <owl:onProperty rdf:resource="http://www.semanticweb.org/hmoudden/ontologies/2022/10/tp01#aGenre"/>
                <owl:qualifiedCardinality rdf:datatype="http://www.w3.org/2001/XMLSchema#nonNegativeInteger">1</owl:qualifiedCardinality>
                <owl:onClass rdf:resource="http://www.semanticweb.org/hmoudden/ontologies/2022/10/tp01#Genre"/>
            </owl:Restriction>
        </rdfs:subClassOf>
        <rdfs:comment xml:lang="en">Person is a class that a person contains different types of Person.
A person necessarily has a gender.
As well as this class allows to have labels by languages and comments for each subclass.</rdfs:comment>
        <rdfs:label xml:lang="en">Person</rdfs:label>
        <rdfs:label xml:lang="fr">Personne</rdfs:label>
    </owl:Class>
    


    <!-- http://www.semanticweb.org/hmoudden/ontologies/2022/10/tp01#Réalisateur -->

    <owl:Class rdf:about="http://www.semanticweb.org/hmoudden/ontologies/2022/10/tp01#Réalisateur">
        <owl:equivalentClass>
            <owl:Class>
                <owl:intersectionOf rdf:parseType="Collection">
                    <rdf:Description rdf:about="http://www.semanticweb.org/hmoudden/ontologies/2022/10/tp01#Personne"/>
                    <owl:Restriction>
                        <owl:onProperty rdf:resource="http://www.semanticweb.org/hmoudden/ontologies/2022/10/tp01#aRéalisé"/>
                        <owl:minQualifiedCardinality rdf:datatype="http://www.w3.org/2001/XMLSchema#nonNegativeInteger">1</owl:minQualifiedCardinality>
                        <owl:onClass rdf:resource="http://www.semanticweb.org/hmoudden/ontologies/2022/10/tp01#Film"/>
                    </owl:Restriction>
                </owl:intersectionOf>
            </owl:Class>
        </owl:equivalentClass>
        <rdfs:subClassOf rdf:resource="http://www.semanticweb.org/hmoudden/ontologies/2022/10/tp01#Personne"/>
        <rdfs:comment xml:lang="en">This is a person who has directed one or more films.
Since Director is a subclass of Person, it inherits the hasGender object property.
As well as this class allows to have labels by languages and comments for each subclass.</rdfs:comment>
        <rdfs:label xml:lang="en">Director</rdfs:label>
        <rdfs:label xml:lang="fr">Réalisateur</rdfs:label>
    </owl:Class>
    <owl:Axiom>
        <owl:annotatedSource rdf:resource="http://www.semanticweb.org/hmoudden/ontologies/2022/10/tp01#Réalisateur"/>
        <owl:annotatedProperty rdf:resource="http://www.w3.org/2002/07/owl#equivalentClass"/>
        <owl:annotatedTarget>
            <owl:Class>
                <owl:intersectionOf rdf:parseType="Collection">
                    <rdf:Description rdf:about="http://www.semanticweb.org/hmoudden/ontologies/2022/10/tp01#Personne"/>
                    <owl:Restriction>
                        <owl:onProperty rdf:resource="http://www.semanticweb.org/hmoudden/ontologies/2022/10/tp01#aRéalisé"/>
                        <owl:minQualifiedCardinality rdf:datatype="http://www.w3.org/2001/XMLSchema#nonNegativeInteger">1</owl:minQualifiedCardinality>
                        <owl:onClass rdf:resource="http://www.semanticweb.org/hmoudden/ontologies/2022/10/tp01#Film"/>
                    </owl:Restriction>
                </owl:intersectionOf>
            </owl:Class>
        </owl:annotatedTarget>
        <rdfs:comment xml:lang="fr">Cette contrainte signifie qu&apos;une personne est un réalisateur si et seulement si elle a réalisé au moins un film.</rdfs:comment>
    </owl:Axiom>
    


    <!-- http://www.semanticweb.org/hmoudden/ontologies/2022/10/tp01#Ville -->

    <owl:Class rdf:about="http://www.semanticweb.org/hmoudden/ontologies/2022/10/tp01#Ville">
        <rdfs:subClassOf rdf:resource="http://www.semanticweb.org/hmoudden/ontologies/2022/10/tp01#Lieu"/>
        <rdfs:comment xml:lang="en">The City is declared as an equivalence class to avoid that a place equivalent to a city is not.
As well as this class allows to have labels by languages.
This class is disjoint with the Continent and Country class, which means that a City cannot be a Continent or a Country.</rdfs:comment>
        <rdfs:label xml:lang="en">City</rdfs:label>
        <rdfs:label xml:lang="fr">Ville</rdfs:label>
    </owl:Class>
    


    <!-- 
    ///////////////////////////////////////////////////////////////////////////////////////
    //
    // Individuals
    //
    ///////////////////////////////////////////////////////////////////////////////////////
     -->

    


    <!-- http://www.semanticweb.org/hmoudden/ontologies/2022/10/tp01#Bérénice_Bejo -->

    <owl:NamedIndividual rdf:about="http://www.semanticweb.org/hmoudden/ontologies/2022/10/tp01#Bérénice_Bejo">
        <rdf:type rdf:resource="http://www.semanticweb.org/hmoudden/ontologies/2022/10/tp01#Personne"/>
        <aGenre rdf:resource="http://www.semanticweb.org/hmoudden/ontologies/2022/10/tp01#Féminin"/>
        <joueDansFilm rdf:resource="http://www.semanticweb.org/hmoudden/ontologies/2022/10/tp01#The_Artist"/>
    </owl:NamedIndividual>
    


    <!-- http://www.semanticweb.org/hmoudden/ontologies/2022/10/tp01#Europe -->

    <owl:NamedIndividual rdf:about="http://www.semanticweb.org/hmoudden/ontologies/2022/10/tp01#Europe">
        <rdf:type rdf:resource="http://www.semanticweb.org/hmoudden/ontologies/2022/10/tp01#Continent"/>
        <rdfs:label xml:lang="en">Europe</rdfs:label>
        <rdfs:label xml:lang="fr">Europe</rdfs:label>
    </owl:NamedIndividual>
    


    <!-- http://www.semanticweb.org/hmoudden/ontologies/2022/10/tp01#France -->

    <owl:NamedIndividual rdf:about="http://www.semanticweb.org/hmoudden/ontologies/2022/10/tp01#France">
        <rdf:type rdf:resource="http://www.semanticweb.org/hmoudden/ontologies/2022/10/tp01#Pays"/>
        <aCapitale rdf:resource="http://www.semanticweb.org/hmoudden/ontologies/2022/10/tp01#Paris"/>
        <situéDans rdf:resource="http://www.semanticweb.org/hmoudden/ontologies/2022/10/tp01#Europe"/>
        <rdfs:label xml:lang="en">France</rdfs:label>
        <rdfs:label xml:lang="fr">France</rdfs:label>
    </owl:NamedIndividual>
    


    <!-- http://www.semanticweb.org/hmoudden/ontologies/2022/10/tp01#Français -->

    <owl:NamedIndividual rdf:about="http://www.semanticweb.org/hmoudden/ontologies/2022/10/tp01#Français">
        <rdf:type rdf:resource="http://www.semanticweb.org/hmoudden/ontologies/2022/10/tp01#Nationalité"/>
        <rdfs:label xml:lang="fr">Français</rdfs:label>
        <rdfs:label xml:lang="en">French</rdfs:label>
    </owl:NamedIndividual>
    


    <!-- http://www.semanticweb.org/hmoudden/ontologies/2022/10/tp01#Féminin -->

    <owl:NamedIndividual rdf:about="http://www.semanticweb.org/hmoudden/ontologies/2022/10/tp01#Féminin">
        <rdf:type rdf:resource="http://www.semanticweb.org/hmoudden/ontologies/2022/10/tp01#Genre"/>
        <rdfs:label xml:lang="en">Female</rdfs:label>
        <rdfs:label xml:lang="fr">Féminin</rdfs:label>
    </owl:NamedIndividual>
    


    <!-- http://www.semanticweb.org/hmoudden/ontologies/2022/10/tp01#Jean_Dujardin -->

    <owl:NamedIndividual rdf:about="http://www.semanticweb.org/hmoudden/ontologies/2022/10/tp01#Jean_Dujardin">
        <rdf:type rdf:resource="http://www.semanticweb.org/hmoudden/ontologies/2022/10/tp01#Personne"/>
        <aGenre rdf:resource="http://www.semanticweb.org/hmoudden/ontologies/2022/10/tp01#Masculin"/>
        <joueDansFilm rdf:resource="http://www.semanticweb.org/hmoudden/ontologies/2022/10/tp01#The_Artist"/>
    </owl:NamedIndividual>
    


    <!-- http://www.semanticweb.org/hmoudden/ontologies/2022/10/tp01#Masculin -->

    <owl:NamedIndividual rdf:about="http://www.semanticweb.org/hmoudden/ontologies/2022/10/tp01#Masculin">
        <rdf:type rdf:resource="http://www.semanticweb.org/hmoudden/ontologies/2022/10/tp01#Genre"/>
        <rdfs:label xml:lang="en">Male</rdfs:label>
        <rdfs:label xml:lang="fr">Masculin</rdfs:label>
    </owl:NamedIndividual>
    


    <!-- http://www.semanticweb.org/hmoudden/ontologies/2022/10/tp01#Michel_Hazanavicius -->

    <owl:NamedIndividual rdf:about="http://www.semanticweb.org/hmoudden/ontologies/2022/10/tp01#Michel_Hazanavicius">
        <rdf:type rdf:resource="http://www.semanticweb.org/hmoudden/ontologies/2022/10/tp01#Personne"/>
        <aGenre rdf:resource="http://www.semanticweb.org/hmoudden/ontologies/2022/10/tp01#Masculin"/>
        <aRéalisé rdf:resource="http://www.semanticweb.org/hmoudden/ontologies/2022/10/tp01#The_Artist"/>
    </owl:NamedIndividual>
    


    <!-- http://www.semanticweb.org/hmoudden/ontologies/2022/10/tp01#Midnight_In_Paris -->

    <owl:NamedIndividual rdf:about="http://www.semanticweb.org/hmoudden/ontologies/2022/10/tp01#Midnight_In_Paris">
        <rdf:type rdf:resource="http://www.semanticweb.org/hmoudden/ontologies/2022/10/tp01#Film"/>
        <réaliséPar rdf:resource="http://www.semanticweb.org/hmoudden/ontologies/2022/10/tp01#Woody_Allen"/>
        <seDérouleDans rdf:resource="http://www.semanticweb.org/hmoudden/ontologies/2022/10/tp01#Paris"/>
        <Durée rdf:datatype="http://www.w3.org/2001/XMLSchema#int">94</Durée>
        <Note xml:lang="en">Some words...</Note>
    </owl:NamedIndividual>
    


    <!-- http://www.semanticweb.org/hmoudden/ontologies/2022/10/tp01#Paris -->

    <owl:NamedIndividual rdf:about="http://www.semanticweb.org/hmoudden/ontologies/2022/10/tp01#Paris">
        <rdf:type rdf:resource="http://www.semanticweb.org/hmoudden/ontologies/2022/10/tp01#Ville"/>
        <situéDans rdf:resource="http://www.semanticweb.org/hmoudden/ontologies/2022/10/tp01#France"/>
        <rdfs:label xml:lang="en">Paris</rdfs:label>
        <rdfs:label xml:lang="fr">Paris</rdfs:label>
        <rdfs:label xml:lang="fr">Ville de lumières</rdfs:label>
    </owl:NamedIndividual>
    


    <!-- http://www.semanticweb.org/hmoudden/ontologies/2022/10/tp01#The_Artist -->

    <owl:NamedIndividual rdf:about="http://www.semanticweb.org/hmoudden/ontologies/2022/10/tp01#The_Artist">
        <rdf:type rdf:resource="http://www.semanticweb.org/hmoudden/ontologies/2022/10/tp01#Film"/>
        <aNationalité rdf:resource="http://www.semanticweb.org/hmoudden/ontologies/2022/10/tp01#Français"/>
        <réaliséPar rdf:resource="http://www.semanticweb.org/hmoudden/ontologies/2022/10/tp01#Michel_Hazanavicius"/>
        <Durée rdf:datatype="http://www.w3.org/2001/XMLSchema#int">100</Durée>
        <Note xml:lang="en">Some words...</Note>
    </owl:NamedIndividual>
    


    <!-- http://www.semanticweb.org/hmoudden/ontologies/2022/10/tp01#Woody_Allen -->

    <owl:NamedIndividual rdf:about="http://www.semanticweb.org/hmoudden/ontologies/2022/10/tp01#Woody_Allen">
        <rdf:type rdf:resource="http://www.semanticweb.org/hmoudden/ontologies/2022/10/tp01#Personne"/>
        <aGenre rdf:resource="http://www.semanticweb.org/hmoudden/ontologies/2022/10/tp01#Masculin"/>
        <aRéalisé rdf:resource="http://www.semanticweb.org/hmoudden/ontologies/2022/10/tp01#Midnight_In_Paris"/>
    </owl:NamedIndividual>
    


    <!-- http://www.semanticweb.org/hmoudden/ontologies/2022/10/tp01#_test_Short_Film -->

    <owl:NamedIndividual rdf:about="http://www.semanticweb.org/hmoudden/ontologies/2022/10/tp01#_test_Short_Film">
        <rdf:type rdf:resource="http://www.semanticweb.org/hmoudden/ontologies/2022/10/tp01#Film"/>
        <Durée rdf:datatype="http://www.w3.org/2001/XMLSchema#int">30</Durée>
    </owl:NamedIndividual>
</rdf:RDF>



<!-- Generated by the OWL API (version 4.5.9.2019-02-01T07:24:44Z) https://github.com/owlcs/owlapi -->

